PlutusCore/Bitwise/Lemmas.lean
@@ -9,18 +9,6 @@ namespace PlutusCore.Bitwise
 
 def Except.isError (e : Except ε α) : Bool := not (Except.isOk e)
 
-example : integerToByteString false 5 0x123456 = .ok "\x56\x34\x12\x00\x00" := rfl
-example : integerToByteString false 4 0x123456 = .ok "\x56\x34\x12\x00"     := rfl
-example : integerToByteString false 3 0x123456 = .ok "\x56\x34\x12"         := rfl
-example : integerToByteString false 2 0x123456 |> Except.isError            := rfl
-example : integerToByteString false 0 0x00     = .ok ""                     := by simp [integerLog2] ; rfl
-
-example : integerToByteString true  5 0x123456 = .ok "\x00\x00\x12\x34\x56" := rfl
-example : integerToByteString true  4 0x123456 = .ok     "\x00\x12\x34\x56" := rfl
-example : integerToByteString true  3 0x123456 = .ok         "\x12\x34\x56" := rfl
-example : integerToByteString true  2 0x123456 |> Except.isError            := rfl
-example : integerToByteString true  0 0x00     = .ok ""                     := by simp [integerLog2]; rfl
-
 -- itobs_be_loop (w, n) = ×, if 256 ^ w ≤ n
 /-- Given `w` and `n`, if 256 ^ w ≤ n, `itobs_be_loop` returns an error -/
 theorem itobs_be_loop_high_n (w n : Nat) (a : List Char) (hwn : 256 ^ w ≤ n) :
@@ -34,21 +22,6 @@ theorem itobs_be_loop_high_n (w n : Nat) (a : List Char) (hwn : 256 ^ w ≤ n) :
       simp [itobs_be_loop]
       rw [ih]
       omega
-
-/-- `repr256_le a` returns `n`, if `a` is the little-endian representation of `n`. -/
-def repr256_le (a : List Char) : Nat :=
-   a |> List.mapIdx (λ i c => (Char.toNat c) * 256 ^ i) |> List.sum
-
-example : repr256_le (String.toList "\x56\x34\x12\x00\x00") = 0x123456 := rfl
-example : repr256_le (String.toList "\x56\x34\x12\x00"    ) = 0x123456 := rfl
-example : repr256_le (String.toList "\x56\x34\x12"        ) = 0x123456 := rfl
-
-/-- `repr256_be a` returns `n`, if `a` is the big-endian representation of `n`. -/
-def repr256_be (a : List Char) : Nat := repr256_le (List.reverse a)
-
-example : repr256_be (String.toList "\x00\x00\x12\x34\x56") = 0x123456 := rfl
-example : repr256_be (String.toList     "\x00\x12\x34\x56") = 0x123456 := rfl
-example : repr256_be (String.toList         "\x12\x34\x56") = 0x123456 := rfl
 
 /-- Lemma usable to drive induction via the base 256 representation of a Nat. -/
 theorem base256_ind (P : Nat → Prop) (h0 : P 0) (hstep : ∀ (q r : Nat), r < 256 → P q → P (256 * q + r)) : ∀ n, P n := by
@@ -296,73 +269,7 @@ theorem itobs_bstoi_equivalence (e : Bool) (s : String) (w n : Integer) :
 theorem bstoi_itobs_equivalence (e : Bool) (s : String) (w n : Integer) :
   w = 0 ∨ String.length s ≤ w → byteStringToInteger e s = n → integerToByteString e w n = .ok s := sorry
 
-example : andByteString true  "\xA5\xFF" "\x5A" = "\x00\xFF" := rfl
-example : andByteString false "\xA5\xFF" "\x5A" = "\x00"     := rfl
-
--- TODO: formalizations for andByteString
-
-example :  orByteString true  "\xA5\xFF" "\x5A" = "\xFF\xFF" := rfl
-example :  orByteString false "\xA5\xFF" "\x5A" = "\xFF"     := rfl
-
--- TODO: formalizations for orByteString
-
-example : xorByteString true  "\xAF\xFF" "\x5A" = "\xF5\xFF" := rfl
-example : xorByteString false "\xAF\xFF" "\x5A" = "\xF5"     := rfl
-
--- TODO: formalizations for xorByteString
-
-example : complementByteString "\xA5\x5F" = "\x5A\xA0" := by native_decide
-
--- TODO: formalizations for complementByteString
-
-example : shiftByteString "\xA5\x5F"   1  = "\x4A\xBE" := rfl
-example : shiftByteString "\xCA\xFE"   4  = "\xAF\xE0" := rfl
-example : shiftByteString "\xCA\xFE" (-4) = "\x0C\xAF" := rfl
-
--- TODO: formalizations for shiftByteString
-
-example : rotateByteString "\xA5\x5F"   1  = "\x4A\xBF" := rfl
-example : rotateByteString "\xCA\xFE"   4  = "\xAF\xEC" := rfl
-example : rotateByteString "\xCA\xFE" (-4) = "\xEC\xAF" := rfl
-
--- TODO: formalizations for rotateByteString
-
-example : countSetBits "\xF0"     = 4 := rfl
-example : countSetBits "\xA5"     = 4 := rfl
-example : countSetBits "\xFF\x00" = 8 := rfl
-
--- TODO: formalizations for countSetBits
-
-example : findFirstSetBit "\xF0"     = 4 := rfl
-example : findFirstSetBit "\xFF\x00" = 8 := rfl
-example : findFirstSetBit "\xFF\x01" = 0 := rfl
-
--- TODO: formalizations for firstSetBit
-
-example : readBit "\xA5"      8 = .error "readBit: index out of bounds" := rfl
-example : readBit "\xA5"      3 = .ok false                             := rfl
-example : readBit "\xA5"      7 = .ok true                              := rfl
-example : readBit "\xA5\x00"  3 = .ok false                             := rfl
-example : readBit "\xA5\x00" 14 = .ok false                             := rfl
-example : readBit "\xA5\x00" 15 = .ok true                              := rfl
-
--- TODO: formalizations for readBit
-
-example : writeBit "\x00\x00"  0 true  = .ok "\x00\x01" := rfl
-example : writeBit "\x00\x01"  0 true  = .ok "\x00\x01" := rfl
-example : writeBit "\x00\x01" 15 true  = .ok "\x80\x01" := rfl
-example : writeBit "\x80\x01"  0 false = .ok "\x80\x00" := rfl
-
--- TODO: formalizations for writeBit
-
-example : writeBits "\x00\x00" [15, 13, 8, 10]    true  = .ok "\xA5\x00" := rfl
-example : writeBits "\x00\x00" [15, 13, 8, 10]    false = .ok "\x00\x00" := rfl
-example : writeBits "\xFF\xFF" [0, 13, 12, 8, 10] false = .ok "\xCA\xFE" := rfl
-
 -- TODO: formalizations for writeBits
-
-example : replicateByte    4 101 = .ok "eeee" := rfl
-example : replicateByte (-4) 101 = .error "replicateByte: negative length requested" := rfl
 
 theorem replicateByte_zero_l (b : Integer) : 0 ≤ b → b ≤ 255 → replicateByte 0 b = .ok "" := by
   intros hbi hbs
