Lemmas.lean
@@ -1,0 +1,3 @@
+-- This module serves as the root of the `Lemmas` library.
+-- Import modules here that should be built as part of the library.
+import Lemmas.Basic
