Lemmas/Basic.lean
@@ -1,0 +1,22 @@
+
+import PlutusCore.Bitwise.Lemmas
+import PlutusCore.Bool.Lemmas
+import PlutusCore.ByteString.Lemmas
+import PlutusCore.Cbor.Lemmas
+import PlutusCore.Crypto.BLS12_381.LemmasG1
+import PlutusCore.Crypto.BLS12_381.LemmasG2
+import PlutusCore.Crypto.BLS12_381.LemmasPairing
+import PlutusCore.Crypto.Ed25519.Lemmas
+import PlutusCore.Crypto.ExpMod.Lemmas
+import PlutusCore.Crypto.Hash.Lemmas
+import PlutusCore.Crypto.Secp256k1.Lemmas
+import PlutusCore.Data.Lemmas
+import PlutusCore.Integer.Lemmas
+import PlutusCore.List.Lemmas
+import PlutusCore.Pair.Lemmas
+import PlutusCore.String.Lemmas
+import PlutusCore.Trace.Lemmas
+import PlutusCore.UPLC.FlatEncoding.Lemmas
+import PlutusCore.UPLC.ScriptEncoding.Lemmas
+import PlutusCore.Unit.Lemmas
+
