PlutusCore/Bitwise.lean
@@ -1,5 +1,4 @@
 
 import PlutusCore.Bitwise.Basic
-import PlutusCore.Bitwise.Lemmas
 
 /-! ## Header file introducing Bitwise formalization. -/
