PlutusCore/Bool.lean
@@ -1,5 +1,4 @@
 
 import PlutusCore.Bool.Basic
-import PlutusCore.Bool.Lemmas
 
 /-! ## Header file introducing Bool formalization. -/
