PlutusCore/ByteString.lean
@@ -1,5 +1,4 @@
 
 import PlutusCore.ByteString.Basic
-import PlutusCore.ByteString.Lemmas
 
 /-! ## Header file introducing ByteString formalization. -/
