PlutusCore/Cbor.lean
@@ -1,5 +1,4 @@
 
 import PlutusCore.Cbor.Basic
-import PlutusCore.Cbor.Lemmas
 
 /-! ## Header file introducing Cbor formalization. -/
