PlutusCore/Crypto/Ed25519.lean
@@ -1,5 +1,4 @@
 
 import PlutusCore.Crypto.Ed25519.Basic
-import PlutusCore.Crypto.Ed25519.Lemmas
 
 /-! ## Header file regrouping the PlutusCore Ed25519 formalization. -/
