PlutusCore/Crypto/ExpMod.lean
@@ -1,4 +1,3 @@
 import PlutusCore.Crypto.ExpMod.Basic
-import PlutusCore.Crypto.ExpMod.Lemmas
 
 /-! ## Header file regrouping the PlutusCore ExpMod formalization. -/
