PlutusCore/Crypto/Hash.lean
@@ -1,5 +1,4 @@
 
 import PlutusCore.Crypto.Hash.Basic
-import PlutusCore.Crypto.Hash.Lemmas
 
 /-! ## Header file regrouping the PlutusCore Hash formalization. -/
