PlutusCore/Crypto/Secp256k1.lean
@@ -1,5 +1,4 @@
 
 import PlutusCore.Crypto.Secp256k1.Basic
-import PlutusCore.Crypto.Secp256k1.Lemmas
 
 /-! ## Header file regrouping the PlutusCore Secp256k1 formalization. -/
