PlutusCore/Data.lean
@@ -1,5 +1,4 @@
 
 import PlutusCore.Data.Basic
-import PlutusCore.Data.Lemmas
 
 /-! ## Header file introducing Data formalization. -/
