PlutusCore/Integer.lean
@@ -1,5 +1,4 @@
 
 import PlutusCore.Integer.Basic
-import PlutusCore.Integer.Lemmas
 
 /-! ## Header file introducing Integer formalization. -/
