PlutusCore/List.lean
@@ -1,5 +1,4 @@
 
 import PlutusCore.List.Basic
-import PlutusCore.List.Lemmas
 
 /-! ## Header file regrouping the PlutusCore List formalization. -/
