PlutusCore/Pair.lean
@@ -1,5 +1,4 @@
 
 import PlutusCore.Pair.Basic
-import PlutusCore.Pair.Lemmas
 
 /-! ## Header file regrouping the PlutusCore Pair formalization. -/
