PlutusCore/String.lean
@@ -1,5 +1,4 @@
 
 import PlutusCore.String.Basic
-import PlutusCore.String.Lemmas
 
 /-! ## Header file regrouping the PlutusCore String formalization. -/
