PlutusCore/Trace.lean
@@ -1,5 +1,4 @@
 
 import PlutusCore.Trace.Basic
-import PlutusCore.Trace.Lemmas
 
 /-! ## Header file regrouping the PlutusCore Trace formalization. -/
