PlutusCore/UPLC/FlatEncoding.lean
@@ -1,3 +1,2 @@
 
 import PlutusCore.UPLC.FlatEncoding.Basic
-import PlutusCore.UPLC.FlatEncoding.Lemmas
