PlutusCore/UPLC/ScriptEncoding.lean
@@ -1,3 +1,2 @@
 
 import PlutusCore.UPLC.ScriptEncoding.Basic
-import PlutusCore.UPLC.ScriptEncoding.Lemmas
