PlutusCore/Unit.lean
@@ -1,5 +1,4 @@
 
 import PlutusCore.Unit.Basic
-import PlutusCore.Unit.Lemmas
 
 /-! ## Header file regrouping the PlutusCore Unit formalization. -/
