lakefile.lean
@@ -4,5 +4,13 @@ open Lake DSL
 package «PlutusCore» where
   -- add package configuration options here
 
+@[default_target]
 lean_lib «PlutusCore» where
+  -- add library configuration options here
+
+@[test_driver]
+lean_lib «Tests» where
+  -- add library configuration options here
+
+lean_lib «Lemmas» where
   -- add library configuration options here
